add binary search

dafny/src/libs/math.dfy
@@ -1,8 +1,11 @@
 module Math {
 
-    const WAD: nat := 1_000_000_000_000_000_000 // 18 zeros
-    const RAY: nat := 1_000_000_000_000_000_000_000_000_000 // 27
-    const PER: nat := 10_000
+    const TWO_256 : int := 0x1_0000_0000_0000_0000_0000_0000_0000_0000_0000_0000_0000_0000_0000_0000_0000_0000
+    const WAD:      nat := 1_000_000_000_000_000_000 // 18 zeros
+    const RAY:      nat := 1_000_000_000_000_000_000_000_000_000 // 27
+    const PERCENT:  nat := 1_000_000_000_000_000_000 // 18 zeros
+    const YEAR: nat := 30758400 // year in seconds
+    const MAX_U256: int := TWO_256 - 1
 
     function Max(x: nat, y: nat) : nat {
         if x > y then x
@@ -14,22 +17,50 @@ module Math {
                  else y
     }
 
-    function MulDivUp(x:nat, y:nat, z:nat) : nat{
-        x
+    /// Returns `ceil(x * y / d)`. [arredonda para cima]
+    /// Reverts if `x * y` overflows, or `d` is zero.
+    //  z := add(iszero(iszero(mod(mul(x, y), d))), div(mul(x, y), d))
+    function MulDivUp(x:nat, y:nat, z:nat) : (r: nat)
+    requires z > 0
+    ensures r == (x * y + z - 1) / z{
+        (x * y + z - 1) / z
     }
 
-    function MulDivDown(x:nat, y:nat, z:nat) : nat{
-        x
+    /// @dev Returns `floor(x * y / d)`. [arredonda para baixo]
+    /// Reverts if `x * y` overflows, or `d` is zero.
+    function MulDivDown(x:nat, y:nat, z:nat) : (r: nat)
+    requires z > 0
+    ensures r == (x * y) / z {
+        (x * y) / z
     }
 
-    function ToWad(x:nat) : nat {
-        x * WAD
+    predicate sorted(a: array<int>)
+    reads a {
+        forall j, k :: 0 <= j < k < a.Length ==> a[j] <= a[k]
     }
 
-    // -- HIGH PRECISION ARITHMETIC
+    method BinarySearch(a: array<int>, key: int) returns (index: int)
+    requires sorted(a)
+    ensures 0 <= index ==> index < a.Length && a[index] == key
+    ensures index < 0 ==> forall k :: 0 <= k < a.Length ==> a[k] != key {
 
-    function Bps(x: nat, y: nat) : (r: nat) {
-        x * y / PER
+    var low, high := 0, a.Length;
+        while low < high
+            invariant 0 <= low <= high <= a.Length
+            invariant forall i ::
+            0 <= i < a.Length && !(low <= i < high) ==> a[i] != key {
+            var mid := (low + high) / 2;
+            if a[mid] < key {
+                low := mid + 1;
+            }
+            else if key < a[mid] {
+                high := mid;
+            }
+            else {
+                return mid;
+            }
+        }
+        return -1;
     }
 
     //rounds to zero if x*y < WAD / 2
@@ -48,5 +79,30 @@ module Math {
         z / y
     }
 
+    function ToWad(x:nat) : nat {
+        x * WAD
+    }
+
+
+}
+
+// -------  TESTS
+
+
+import opened Math
+method TestDiv1() {
+    assert MulDivUp(7, 3, 4) == 6;
+    assert MulDivUp(3, 5, 4) == 4;
+    assert MulDivUp(4, 5, 4) == 5;
+
+}
+method TestDiv2() {
+    assert MulDivUp(10, 5, 2) == 25;
+    assert MulDivUp(15, 1, 2) == 8;
+}
+method TestDiv3() {
+    assert MulDivDown(7, 3, 4) == 5;
+    assert MulDivDown(3, 5, 4) == 3;
+    assert MulDivDown(4, 5, 4) == 5;
 }
 
